Add pack and unpack methods, which resolve to peekArray and pokeArray

src/Heap.v
@@ -24,6 +24,55 @@ Definition peekS    := "peek".
 Definition pokeS    := "poke".
 Definition memcpyS  := "memcpy".
 Definition memsetS  := "memset".
+Definition readS    := "read".
+Definition writeS   := "write".
+
+Definition fold_left_index
+           {A B} (f : A -> N -> B -> A) (xs : list B) (n : N) (z : A) : A :=
+  fst (fold_left (fun (acc : A * N) x =>
+                    let (m, i) := acc in (f m i x, N.succ i)) xs (z, n)).
+
+Definition load_into_map {elt} (k : M.key) (xs : list elt) (m : M.t elt) :=
+  fold_left_index (fun m i x => M.add (plusPtr (A:=M.key) k i) x m) xs 0 m.
+
+Lemma fold_left_index_cons : forall A B f xs n (a : A) (m : B),
+  fold_left_index f (a :: xs) n m = fold_left_index f xs (N.succ n) (f m n a).
+Proof.
+  induction xs; simpl; intros.
+    reflexivity.
+  rewrite IHxs; clear IHxs.
+  unfold fold_left_index; simpl.
+  reflexivity.
+Qed.
+
+Lemma Equal_fold_left_index :
+  forall elt (addr : Ptr Word) xs n (x y : M.t elt),
+    M.Equal x y ->
+    M.Equal (fold_left_index (fun m i x => M.add (plusPtr addr i) x m) xs n x)
+            (fold_left_index (fun m i x => M.add (plusPtr addr i) x m) xs n y).
+Proof.
+  intros.
+  generalize dependent n.
+  generalize dependent x.
+  generalize dependent y.
+  induction xs; simpl; intros.
+    unfold fold_left_index; simpl.
+    assumption.
+  rewrite !fold_left_index_cons.
+  apply IHxs; eauto.
+  rewrite H.
+  reflexivity.
+Qed.
+
+Lemma load_into_map_Proper {elt} :
+  Proper (N.eq ==> eq ==> @M.Equal elt ==> @M.Equal elt) (@load_into_map elt).
+Proof.
+  relational.
+  unfold load_into_map.
+  rewrite H.
+  apply Equal_fold_left_index.
+  assumption.
+Qed.
 
 Definition HeapSpec := Def ADT {
   (* Map of memory addresses to blocks, which contain another mapping from
@@ -86,7 +135,21 @@ Definition HeapSpec := Def ADT {
          ; bytes := P.update (bytes r)
                              (N.peano_rect
                                 (fun _ => M.t Word) (bytes r)
-                                (fun i => M.add (plusPtr addr i)%N w) len) |}
+                                (fun i => M.add (plusPtr addr i)%N w) len) |},
+
+  Def Method2 readS (r : rep) (addr : Ptr Word) (len : Size) : rep * (list Word) :=
+    xs <- { xs : list Word
+          | xs = N.peano_rect
+                   (fun _ => list Word) []%list
+                   (fun i xs => match M.find (plusPtr addr i) (bytes r) with
+                                | None   => Zero
+                                | Some w => w
+                                end :: xs) len };
+    ret (r, xs),
+
+  Def Method2 writeS (r : rep) (addr : Ptr Word) (xs : list Word) : rep :=
+    ret {| resvs := resvs r
+         ; bytes := load_into_map addr xs (bytes r) |}
 
 }%ADTParsing.
 
@@ -130,6 +193,16 @@ Definition memset (r : Rep HeapSpec)
            (addr : Ptr Word) (len : Ptr Word) (w : Word) :
   Comp (Rep HeapSpec) :=
   Eval simpl in callMeth HeapSpec memsetS r addr len w.
+
+Definition read (r : Rep HeapSpec)
+           (addr : Ptr Word) (len : Ptr Word) :
+  Comp (Rep HeapSpec * list Word) :=
+  Eval simpl in callMeth HeapSpec readS r addr len.
+
+Definition write (r : Rep HeapSpec)
+           (addr : Ptr Word) (xs : list Word) :
+  Comp (Rep HeapSpec) :=
+  Eval simpl in callMeth HeapSpec writeS r addr xs.
 
 (**
  ** Theorems related to the Heap specification.
